almost done

dev2015/dot-smallstep4.v
@@ -1,5 +1,5 @@
 (* smallstep proof *)
-(* compared to 3b, makes tobj recursive (still only one member) *)
+(* compared to 3c, it adds multiple members *)
 
 Require Export SfLib.
 
@@ -9,31 +9,43 @@ Require Export Arith.Lt.
 Module STLC.
 
 Definition id := nat.
+Definition lb := nat.
 
 Inductive ty : Type :=
   | TBot   : ty
   | TTop   : ty
-  | TFun   : ty -> ty -> ty
-  | TMem   : ty -> ty -> ty (* intro *)
+  | TFun   : lb -> ty -> ty -> ty
+  | TMem   : lb -> ty -> ty -> ty (* intro *)
   | TVar   : bool -> id -> ty
   | TVarB  : id -> ty                   
-  | TSel   : ty -> ty (* elim *)
+  | TSel   : ty -> lb -> ty (* elim *)
   | TBind  : ty -> ty
   | TAnd   : ty -> ty -> ty
 .
 
 Inductive tm : Type :=
   | tvar  : bool -> id -> tm
-  | tobj  : dm -> tm (* todo: multiple members *)
-  | tapp  : tm -> tm -> tm
+  | tobj  : dms -> tm
+  | tapp  : tm -> lb -> tm -> tm
 
 with dm : Type :=
   | dfun : ty -> ty -> tm -> dm
   | dty  : ty -> dm
+
+(* we need our own list-like structure for stuctural recursion, e.g. in subst_tm *)
+with dms : Type :=
+  | dnil : dms
+  | dcons : dm -> dms -> dms
 .
 
+Fixpoint dms_to_list (ds: dms) : list dm :=
+  match ds with
+    | dnil => []
+    | dcons d ds => d :: dms_to_list ds
+  end.
+
 Inductive vl : Type :=
-  | vobj  : dm -> vl
+  | vobj  : dms -> vl
 .
 
 Definition venv := list vl.
@@ -54,14 +66,14 @@ Inductive closed: nat -> nat -> nat -> ty -> Prop :=
     closed i j k TBot
 | cl_top: forall i j k,
     closed i j k TTop
-| cl_fun: forall i j k T1 T2,
+| cl_fun: forall i j k l T1 T2,
     closed i j k T1 ->
     closed i j (S k) T2 ->
-    closed i j k (TFun T1 T2)
-| cl_mem: forall i j k T1 T2,
+    closed i j k (TFun l T1 T2)
+| cl_mem: forall i j k l T1 T2,
     closed i j k T1 ->
     closed i j k T2 ->        
-    closed i j k (TMem T1 T2)
+    closed i j k (TMem l T1 T2)
 | cl_var0: forall i j k x,
     i > x ->
     closed i j k (TVar false x)
@@ -71,9 +83,9 @@ Inductive closed: nat -> nat -> nat -> ty -> Prop :=
 | cl_varB: forall i j k x,
     k > x ->
     closed i j k (TVarB x)
-| cl_sel: forall i j k T1,
+| cl_sel: forall i j k T1 l,
     closed i j k T1 ->
-    closed i j k (TSel T1)
+    closed i j k (TSel T1 l)
 | cl_bind: forall i j k T1,
     closed i j (S k) T1 ->
     closed i j k (TBind T1)
@@ -90,9 +102,9 @@ Fixpoint open (k: nat) (u: ty) (T: ty) { struct T }: ty :=
     | TVarB x => if beq_nat k x then u else TVarB x
     | TTop        => TTop
     | TBot        => TBot
-    | TSel T1     => TSel (open k u T1)                  
-    | TFun T1 T2  => TFun (open k u T1) (open (S k) u T2)
-    | TMem T1 T2  => TMem (open k u T1) (open k u T2)
+    | TSel T1 l     => TSel (open k u T1) l
+    | TFun l T1 T2  => TFun l (open k u T1) (open (S k) u T2)
+    | TMem l T1 T2  => TMem l (open k u T1) (open k u T2)
     | TBind T1    => TBind (open (S k) u T1)
     | TAnd T1 T2  => TAnd (open k u T1) (open k u T2)
   end.
@@ -101,12 +113,12 @@ Fixpoint subst (U : ty) (T : ty) {struct T} : ty :=
   match T with
     | TTop         => TTop
     | TBot         => TBot
-    | TMem T1 T2   => TMem (subst U T1) (subst U T2)
-    | TSel T1      => TSel (subst U T1)
+    | TMem l T1 T2 => TMem l (subst U T1) (subst U T2)
+    | TSel T1 l    => TSel (subst U T1) l
     | TVarB i      => TVarB i
     | TVar true i  => TVar true i
     | TVar false i => if beq_nat i 0 then U else TVar false (i-1)
-    | TFun T1 T2   => TFun (subst U T1) (subst U T2)
+    | TFun l T1 T2 => TFun l (subst U T1) (subst U T2)
     | TBind T2     => TBind (subst U T2)
     | TAnd T1 T2   => TAnd (subst U T1) (subst U T2)
   end.
@@ -116,13 +128,18 @@ Fixpoint subst_tm (u:nat) (T : tm) {struct T} : tm :=
   match T with
     | tvar true i         => tvar true i
     | tvar false i        => if beq_nat i 0 then (tvar true u) else tvar false (i-1)
-    | tobj ds             => tobj (subst_dm u ds)
-    | tapp t1 t2          => tapp (subst_tm u t1) (subst_tm u t2)
+    | tobj ds             => tobj (subst_dms u ds)
+    | tapp t1 l t2          => tapp (subst_tm u t1) l (subst_tm u t2)
   end
 with subst_dm (u:nat) (d: dm) {struct d} : dm :=
   match d with
     | dty T        => dty (subst (TVar true u) T)
     | dfun T1 T2 t => dfun (subst (TVar true u) T1) (subst (TVar true u) T2) (subst_tm u t)
+  end
+with subst_dms (u:nat) (ds: dms) {struct ds} : dms :=
+  match ds with
+    | dnil        => dnil
+    | dcons d ds1  => dcons (subst_dm u d) (subst_dms u ds1)
   end.
 
 Definition substt x T := (subst (TVar true x) T).
@@ -132,7 +149,7 @@ Inductive has_type : tenv -> venv -> tm -> ty -> nat -> Prop :=
   | T_Varx : forall GH G1 x ds ds' T T' n1,
       index x G1 = Some (vobj ds) ->
       dms_has_type [T'] G1 ds' T' n1 ->
-      subst_dm x ds' = ds ->
+      subst_dms x ds' = ds ->
       substt x T' = T ->
       closed 0 (length G1) 0 T ->
       has_type GH G1 (tvar true x) T (S n1)
@@ -155,32 +172,39 @@ Inductive has_type : tenv -> venv -> tm -> ty -> nat -> Prop :=
       closed (length GH) (length G1) 1 T ->
       T' = open 0 (TVar false (length GH)) T ->
       has_type GH G1 (tobj ds) (TBind T) (S n1)
-  | T_App : forall T1 T2 GH G1 t1 t2 n1 n2,
-      has_type GH G1 t1 (TFun T1 T2) n1 ->
+  | T_App : forall l T1 T2 GH G1 t1 t2 n1 n2,
+      has_type GH G1 t1 (TFun l T1 T2) n1 ->
       has_type GH G1 t2 T1 n2 ->
       closed (length GH) (length G1) 0 T2 ->
-      has_type GH G1 (tapp t1 t2) T2 (S (n1+n2))
-  | T_AppVar : forall T1 T2 T2' GH G1 t1 b2 x2 n1 n2,
-      has_type GH G1 t1 (TFun T1 T2) n1 ->
+      has_type GH G1 (tapp t1 l t2) T2 (S (n1+n2))
+  | T_AppVar : forall l T1 T2 T2' GH G1 t1 b2 x2 n1 n2,
+      has_type GH G1 t1 (TFun l T1 T2) n1 ->
       has_type GH G1 (tvar b2 x2) T1 n2 ->
       T2' = (open 0 (TVar b2 x2) T2) ->
       closed (length GH) (length G1) 0 T2' ->
-      has_type GH G1 (tapp t1 (tvar b2 x2)) T2' (S (n1+n2))
+      has_type GH G1 (tapp t1 l (tvar b2 x2)) T2' (S (n1+n2))
   | T_Sub : forall GH G1 t T1 T2 n1 n2,
       has_type GH G1 t T1 n1 ->
       stp2 GH G1 T1 T2 n2 ->
       has_type GH G1 t T2 (S (n1 + n2))
-(* todo: multiple members *)
-with dms_has_type: tenv -> venv -> dm -> ty -> nat -> Prop :=
-  | D_Mem : forall GH G1 T11 n1,
+with dms_has_type: tenv -> venv -> dms -> ty -> nat -> Prop :=
+  | D_Nil : forall GH G1 n1,
+      dms_has_type GH G1 dnil TTop (S n1)
+  | D_Mem : forall GH G1 l T11 ds TS T n1,
+      dms_has_type GH G1 ds TS n1 ->
       closed (length GH) (length G1) 0 T11 ->
-      dms_has_type GH G1 (dty T11) (TMem T11 T11) (S n1)
-  | D_Abs : forall GH G1 T11 T12 T12' t12 n1,
-      has_type (T11::GH) G1 t12 T12' n1 ->
+      l = length (dms_to_list ds) ->
+      T = TAnd (TMem l T11 T11) TS ->
+      dms_has_type GH G1 (dcons (dty T11) ds) T (S n1)
+  | D_Abs : forall GH G1 l T11 T12 T12' t12 ds TS T n1 n2,
+      dms_has_type GH G1 ds TS n1 ->
+      has_type (T11::GH) G1 t12 T12' n2 ->
       T12' = (open 0 (TVar false (length GH)) T12) ->
       closed (length GH) (length G1) 0 T11 ->
       closed (length GH) (length G1) 1 T12 ->
-      dms_has_type GH G1 (dfun T11 T12 t12) (TFun T11 T12) (S n1)
+      l = length (dms_to_list ds) ->
+      T = TAnd (TFun l T11 T12) TS ->
+      dms_has_type GH G1 (dcons (dfun T11 T12 t12) ds) T (S (n1+n2))
 
 with stp2: tenv -> venv -> ty -> ty -> nat -> Prop :=
 | stp2_bot: forall GH G1 T n1,
@@ -189,18 +213,18 @@ with stp2: tenv -> venv -> ty -> ty -> nat -> Prop :=
 | stp2_top: forall GH G1 T n1,
     closed (length GH) (length G1) 0 T ->
     stp2 GH G1 T  TTop (S n1)
-| stp2_fun: forall GH G1 T1 T2 T3 T4 T2' T4' n1 n2,
+| stp2_fun: forall GH G1 l T1 T2 T3 T4 T2' T4' n1 n2,
     T2' = (open 0 (TVar false (length GH)) T2) ->
     T4' = (open 0 (TVar false (length GH)) T4) ->
     closed (length GH) (length G1) 1 T2 ->
     closed (length GH) (length G1) 1 T4 ->
     stp2 GH G1 T3 T1 n1 ->
     stp2 (T3::GH) G1 T2' T4' n2 ->
-    stp2 GH G1 (TFun T1 T2) (TFun T3 T4) (S (n1+n2))
-| stp2_mem: forall GH G1 T1 T2 T3 T4 n1 n2,
+    stp2 GH G1 (TFun l T1 T2) (TFun l T3 T4) (S (n1+n2))
+| stp2_mem: forall GH G1 l T1 T2 T3 T4 n1 n2,
     stp2 GH G1 T3 T1 n2 ->
     stp2 GH G1 T2 T4 n1 ->
-    stp2 GH G1 (TMem T1 T2) (TMem T3 T4) (S (n1+n2))
+    stp2 GH G1 (TMem l T1 T2) (TMem l T3 T4) (S (n1+n2))
 
 | stp2_varx: forall GH G1 x n1,
     x < length G1 ->
@@ -209,26 +233,28 @@ with stp2: tenv -> venv -> ty -> ty -> nat -> Prop :=
     x < length GH ->
     stp2 GH G1 (TVar false x) (TVar false x) (S n1)
 
-| stp2_strong_sel1: forall GH G1 T2 TX x n1,
-    index x G1 = Some (vobj (dty TX)) ->
+| stp2_strong_sel1: forall GH G1 l T2 ds TX x n1,
+    index x G1 = Some (vobj ds) ->
+    index l (dms_to_list ds) = Some (dty TX) ->
     stp2 [] G1 TX T2 n1 ->
-    stp2 GH G1 (TSel (TVar true x)) T2 (S n1)
-| stp2_strong_sel2: forall GH G1 T1 TX x n1,
-    index x G1 = Some (vobj (dty TX)) ->
+    stp2 GH G1 (TSel (TVar true x) l) T2 (S n1)
+| stp2_strong_sel2: forall GH G1 l T1 ds TX x n1,
+    index x G1 = Some (vobj ds) ->
+    index l (dms_to_list ds) = Some (dty TX) ->
     stp2 [] G1 T1 TX n1 ->
-    stp2 GH G1 T1 (TSel (TVar true x)) (S n1)
+    stp2 GH G1 T1 (TSel (TVar true x) l) (S n1)
 
-| stp2_sel1: forall GH G1 T2 x n1,
-    htp  GH G1 x (TMem TBot T2) n1 ->
-    stp2 GH G1 (TSel (TVar false x)) T2 (S n1)
+| stp2_sel1: forall GH G1 l T2 x n1,
+    htp  GH G1 x (TMem l TBot T2) n1 ->
+    stp2 GH G1 (TSel (TVar false x) l) T2 (S n1)
 
-| stp2_sel2: forall GH G1 T1 x n1,
-    htp  GH G1 x (TMem T1 TTop) n1 ->
-    stp2 GH G1 T1 (TSel (TVar false x)) (S n1)
+| stp2_sel2: forall GH G1 l T1 x n1,
+    htp  GH G1 x (TMem l T1 TTop) n1 ->
+    stp2 GH G1 T1 (TSel (TVar false x) l) (S n1)
 
-| stp2_selx: forall GH G1 T1 n1,
+| stp2_selx: forall GH G1 l T1 n1,
     closed (length GH) (length G1) 0 T1 ->
-    stp2 GH G1 (TSel T1) (TSel T1) (S n1)
+    stp2 GH G1 (TSel T1 l) (TSel T1 l) (S n1)
 
          
 
@@ -290,14 +316,17 @@ with vtp : nat -> venv -> nat -> ty -> nat -> Prop :=
 | vtp_top: forall m G1 x n1,
     x < length G1 ->
     vtp m G1 x TTop (S n1)
-| vtp_mem: forall m G1 x TX T1 T2 n1 n2,
-    index x G1 = Some (vobj (dty TX)) ->
+| vtp_mem: forall m G1 x l ds TX T1 T2 n1 n2,
+    index x G1 = Some (vobj ds) ->
+    index l (dms_to_list ds) = Some (dty TX) ->
     stp2 [] G1 T1 TX n1 ->
     stp2 [] G1 TX T2 n2 ->
-    vtp m G1 x (TMem T1 T2) (S (n1+n2))
-| vtp_fun: forall m G1 x T1 T2 T3 T4 T2' T4' t T1x T2x tx T' T2x' n1 n2 n3 n4,
-    index x G1 = Some (vobj (dfun T1 T2 t)) ->
-    dms_has_type [T'] G1 (dfun T1x T2x tx) T' n4 ->
+    vtp m G1 x (TMem l T1 T2) (S (n1+n2))
+| vtp_fun: forall m G1 x l ds dsx T1 T2 T3 T4 T2' T4' t T1x T2x tx T' T2x' n1 n2 n3 n4,
+    index x G1 = Some (vobj ds) ->
+    index l (dms_to_list ds) = Some (dfun T1 T2 t) ->
+    subst_dms x dsx = ds ->
+    dms_has_type [T'] G1 dsx T' n4 ->
     subst_dm x (dfun T1x T2x tx) = (dfun T1 T2 t) ->
     T2x' = (open 0 (TVar false 1) T2x) ->
     has_type [T1x;T'] G1 tx T2x' n3 ->
@@ -307,15 +336,16 @@ with vtp : nat -> venv -> nat -> ty -> nat -> Prop :=
     closed 0 (length G1) 1 T2 ->
     closed 0 (length G1) 1 T4 ->
     stp2 [T3] G1 T2' T4' n2 ->
-    vtp m G1 x (TFun T3 T4) (S (n1+n2+n3+n4))
+    vtp m G1 x (TFun l T3 T4) (S (n1+n2+n3+n4))
 | vtp_bind: forall m G1 x T2 n1,
     vtp m G1 x (open 0 (TVar true x) T2) n1 ->
     closed 0 (length G1) 1 T2 ->
     vtp (S m) G1 x (TBind T2) (S (n1))
-| vtp_sel: forall m G1 x y TX n1,
-    index y G1 = Some (vobj (dty TX)) ->
+| vtp_sel: forall m G1 x y l ds TX n1,
+    index y G1 = Some (vobj ds) ->
+    index l (dms_to_list ds) = Some (dty TX) ->
     vtp m G1 x TX n1 ->
-    vtp m G1 x (TSel (TVar true y)) (S (n1))
+    vtp m G1 x (TSel (TVar true y) l) (S (n1))
 | vtp_and: forall m m1 m2 G1 x T1 T2 n1 n2,
     vtp m1 G1 x T1 n1 ->
     vtp m2 G1 x T2 n2 ->
@@ -356,19 +386,19 @@ Lemma stpd2_top: forall GH G1 T,
     closed (length GH) (length G1) 0 T ->
     stpd2 GH G1 T TTop.
 Proof. intros. exists 1. eauto. Qed.
-Lemma stpd2_fun: forall GH G1 T1 T2 T3 T4 T2' T4',
+Lemma stpd2_fun: forall GH G1 l T1 T2 T3 T4 T2' T4',
     T2' = (open 0 (TVar false (length GH)) T2) ->
     T4' = (open 0 (TVar false (length GH)) T4) ->
     closed (length GH) (length G1) 1 T2 ->
     closed (length GH) (length G1) 1 T4 ->
     stpd2 GH G1 T3 T1 ->
     stpd2 (T3::GH) G1 T2' T4' ->
-    stpd2 GH G1 (TFun T1 T2) (TFun T3 T4).
+    stpd2 GH G1 (TFun l T1 T2) (TFun l T3 T4).
 Proof. intros. repeat eu. eexists. eauto. Qed.
-Lemma stpd2_mem: forall GH G1 T1 T2 T3 T4,
+Lemma stpd2_mem: forall GH G1 l T1 T2 T3 T4,
     stpd2 GH G1 T3 T1 ->
     stpd2 GH G1 T2 T4 ->
-    stpd2 GH G1 (TMem T1 T2) (TMem T3 T4).
+    stpd2 GH G1 (TMem l T1 T2) (TMem l T3 T4).
 Proof. intros. repeat eu. eexists. eauto. Qed.
 
 
@@ -520,8 +550,8 @@ Proof.
   - econstructor. eapply IHn. eauto. omega. eapply IHn. eauto. omega. 
   - econstructor. simpl. eauto.
   - econstructor. eauto.
-  - econstructor. eapply index_extend. eauto. eapply IHn. eauto. omega.
-  - econstructor. eapply index_extend. eauto. eapply IHn. eauto. omega.
+  - econstructor. eapply index_extend. eauto. eauto. eapply IHn. eauto. omega.
+  - econstructor. eapply index_extend. eauto. eauto. eapply IHn. eauto. omega.
   - econstructor. eapply IHn. eauto. omega.
   - econstructor. eapply IHn. eauto. omega.
   - econstructor. eapply closed_extend. eauto. 
@@ -533,10 +563,10 @@ Proof.
   - eapply stp2_transf. eapply IHn. eauto. omega. eapply IHn. eauto. omega. 
   (* vtp *)    
   - econstructor. simpl. eauto.
-  - econstructor. eapply index_extend. eauto. eapply IHn. eauto. omega. eapply IHn. eauto. omega.
-  - econstructor. eapply index_extend. eauto. eapply IHn. eauto. omega. eauto. eauto. eapply IHn. eauto. omega. eapply IHn. eauto. omega. eauto. eauto. eapply closed_extend. eauto. eapply closed_extend. eauto. eapply IHn. eauto. omega.
+  - econstructor. eapply index_extend. eauto. eauto. eapply IHn. eauto. omega. eapply IHn. eauto. omega.
+  - econstructor. eapply index_extend. eauto. eauto. eauto. eapply IHn. eauto. omega. eauto. eauto. eapply IHn. eauto. omega. eapply IHn. eauto. omega. eauto. eauto. eapply closed_extend. eauto. eapply closed_extend. eauto. eapply IHn. eauto. omega.
   - econstructor. eapply IHn. eauto. omega. eapply closed_extend. eauto. 
-  - econstructor. eapply index_extend. eauto. eapply IHn. eauto. omega.
+  - econstructor. eapply index_extend. eauto. eauto. eapply IHn. eauto. omega.
   - econstructor. eapply IHn. eauto. omega. eapply IHn. eauto. omega. eauto. eauto. 
   (* htp *)
   - econstructor. eauto. eapply closed_extend. eauto. 
@@ -552,8 +582,9 @@ Proof.
   - eapply T_AppVar. eapply IHn. eauto. omega. eapply IHn. eauto. omega. eauto. eapply closed_extend. eauto.
   - econstructor. eapply IHn. eauto. omega. eapply IHn. eauto. omega.
   (* dms_has_type *)
-  - econstructor. eapply closed_extend. eauto.
-  - econstructor. eapply IHn. eauto. omega. eauto. eapply closed_extend. eauto. eapply closed_extend. eauto.
+  - econstructor.
+  - econstructor. eapply IHn. eauto. omega. eapply closed_extend. eauto. eauto. eauto.
+  - econstructor. eapply IHn. eauto. omega. eapply IHn. eauto. omega. eauto. eapply closed_extend. eauto. eapply closed_extend. eauto. eauto. eauto.
 Qed.
 
 Lemma closed_upgrade_gh: forall i i1 j k T1,
@@ -625,7 +656,7 @@ Proof.
   - econstructor. simpl. eauto.
   - econstructor. eauto.
   - econstructor. econstructor. eapply index_max. eauto. 
-  - eapply closed_upgrade_gh. eapply IHS1. eapply H2. omega. simpl. omega.  
+  - eapply closed_upgrade_gh. eapply IHS1. eauto. omega. simpl. omega.
   - econstructor. econstructor. eapply IHH1. eauto. omega.
   - eapply closed_upgrade_gh. eapply IHH2 in H1. inversion H1. eauto. omega. simpl. omega.
   - econstructor. eauto.
@@ -642,7 +673,7 @@ Proof.
   - econstructor. eapply IHS1. eauto. omega. eapply IHS2. eauto. omega. 
   - econstructor. simpl. eauto.
   - econstructor. eauto.
-  - eapply closed_upgrade_gh. eapply IHS2. eapply H2. omega. simpl. omega.  
+  - eapply closed_upgrade_gh. eapply IHS2. eauto. omega. simpl. omega.  
   - econstructor. econstructor. eapply index_max. eauto.
   - eapply closed_upgrade_gh. eapply IHH2 in H1. inversion H1. eauto. omega. simpl. omega.
   - econstructor. econstructor. eapply IHH1. eauto. omega.
@@ -685,8 +716,9 @@ Proof.
   - eapply IHT in H1. inversion H1. eauto. omega.
   - eapply IHS2. eauto. omega.
   (* dms_has_type *)
-  - econstructor. eauto. eauto.
-  - econstructor. eauto. eapply closed_upgrade. eauto. omega.
+  - econstructor.
+  - subst. econstructor. econstructor. eauto. eauto. eapply IHD. eauto. omega.
+  - subst. econstructor. econstructor. eauto. eauto. eapply IHD. eauto. omega.
 Qed.
 
 
@@ -810,9 +842,9 @@ Fixpoint tsize (T: ty) { struct T }: nat :=
     | TVarB x => 1
     | TTop        => 1
     | TBot        => 1
-    | TSel T1     => S (tsize T1)
-    | TFun T1 T2  => S (tsize T1 + tsize T2)
-    | TMem T1 T2  => S (tsize T1 + tsize T2)
+    | TSel T1 l   => S (tsize T1)
+    | TFun l T1 T2 => S (tsize T1 + tsize T2)
+    | TMem l T1 T2 => S (tsize T1 + tsize T2)
     | TBind T1    => S (tsize T1)
     | TAnd T1 T2  => S (tsize T1 + tsize T2)
   end.
@@ -883,10 +915,10 @@ Ltac index_subst := match goal with
 
 Ltac invty := match goal with
                 | H1: TBot     = _ |- _ => inversion H1
-                | H1: TSel _   = _ |- _ => inversion H1
-                | H1: TMem _ _ = _ |- _ => inversion H1
+                | H1: TSel _ _   = _ |- _ => inversion H1
+                | H1: TMem _ _ _ = _ |- _ => inversion H1
                 | H1: TVar _ _ = _ |- _ => inversion H1
-                | H1: TFun _ _ = _ |- _ => inversion H1
+                | H1: TFun _ _ _ = _ |- _ => inversion H1
                 | H1: TBind  _ = _ |- _ => inversion H1
                 | H1: TAnd _ _ = _ |- _ => inversion H1
                 | _ => idtac
@@ -895,8 +927,8 @@ Ltac invty := match goal with
 Ltac invstp_var := match goal with
   | H1: stp2 _ true _ _ TBot        (TVar _ _) _ |- _ => inversion H1
   | H1: stp2 _ true _ _ TTop        (TVar _ _) _ |- _ => inversion H1
-  | H1: stp2 _ true _ _ (TFun _ _)  (TVar _ _) _ |- _ => inversion H1
-  | H1: stp2 _ true _ _ (TMem _ _)  (TVar _ _) _ |- _ => inversion H1
+  | H1: stp2 _ true _ _ (TFun _ _ _)  (TVar _ _) _ |- _ => inversion H1
+  | H1: stp2 _ true _ _ (TMem _ _ _)  (TVar _ _) _ |- _ => inversion H1
   | H1: stp2 _ true _ _ (TAnd _ _)  (TVar _ _) _ |- _ => inversion H1
   | _ => idtac
 end.
@@ -1266,18 +1298,18 @@ Proof.
       repeat eexists. unfold substt. simpl. rewrite E. eapply stp2_varax. rewrite map_length. rewrite app_length in H2. simpl in H2. omega. 
   - Case "ssel1". subst. 
     assert (substt x T2 = T2) as R. eapply subst_closed_id. eapply stpd2_closed2 with (GH:=[]). eauto. 
-    eexists. eapply stp2_strong_sel1. eauto. rewrite R. eauto. 
+    eexists. eapply stp2_strong_sel1. eauto. eauto. rewrite R. eauto. 
     
   - Case "ssel2". subst. 
     assert (substt x T1 = T1) as R. eapply subst_closed_id. eapply stpd2_closed1 with (GH:=[]). eauto. 
-    eexists. eapply stp2_strong_sel2. eauto. rewrite R. eauto. 
+    eexists. eapply stp2_strong_sel2. eauto. eauto. rewrite R. eauto. 
 
   - Case "sel1". subst. (* invert htp to vtp and create strong_sel node *)
     case_eq (beq_nat x0 0); intros E.
     + assert (x0 = 0). eapply beq_nat_true_iff. eauto. subst x0.
-      assert (exists m0, vtpd m0 G1 x (substt x (TMem TBot T2))) as A. eapply narrowX. eauto. omega.
+      assert (exists m0, vtpd m0 G1 x (substt x (TMem l TBot T2))) as A. eapply narrowX. eauto. omega.
       destruct A as [? A]. eu. inversion A. subst.
-      repeat eexists. eapply stp2_strong_sel1. eauto. unfold substt. 
+      repeat eexists. eapply stp2_strong_sel1. eauto. eauto. unfold substt. 
       eauto.
     + assert (x0 <> 0). eapply beq_nat_false_iff. eauto.
       eapply htp_subst_narrow02 in H2. 
@@ -1286,9 +1318,9 @@ Proof.
   - Case "sel2". subst. (* invert htp to vtp and create strong_sel node *)
     case_eq (beq_nat x0 0); intros E.
     + assert (x0 = 0). eapply beq_nat_true_iff. eauto. subst x0.
-      assert (exists m0, vtpd m0 G1 x (substt x (TMem T1 TTop))) as A. eapply narrowX. eauto. omega.
+      assert (exists m0, vtpd m0 G1 x (substt x (TMem l T1 TTop))) as A. eapply narrowX. eauto. omega.
       destruct A as [? A]. eu. inversion A. subst. 
-      repeat eexists. eapply stp2_strong_sel2. eauto. unfold substt. 
+      repeat eexists. eapply stp2_strong_sel2. eauto. eauto. unfold substt. 
       eauto.
     + assert (x0 <> 0). eapply beq_nat_false_iff. eauto.
       eapply htp_subst_narrow02 in H2. 
@@ -1637,7 +1669,7 @@ Proof.
     + SCase "top". repeat eexists; eauto.
     + SCase "ssel2".
       assert (vtpdd m1 G1 x TX). eapply IHn; eauto. omega. 
-      eu. repeat eexists. eapply vtp_sel. eauto. eauto. eauto.
+      eu. repeat eexists. eapply vtp_sel. eauto. eauto. eauto. eauto.
     + SCase "sel2".
       eapply stp2_closed2 in H0. simpl in H0. inversion H0. inversion H9. omega.
     + SCase "and".
@@ -1651,15 +1683,15 @@ Proof.
   - Case "mem". inversion H0; subst; invty.
     + SCase "top". repeat eexists. eapply vtp_top. eapply index_max. eauto. eauto. 
     + SCase "mem". invty. subst.
-      repeat eexists. eapply vtp_mem. eauto.
-      eapply stp2_transf. eauto. eapply H5.
-      eapply stp2_transf. eauto. eapply H13.
+      repeat eexists. eapply vtp_mem. eauto. eauto.
+      eapply stp2_transf. eauto. eauto.
+      eapply stp2_transf. eauto. eauto.
       eauto. 
     + SCase "sel2". 
       assert (vtpdd m1 G1 x TX0). eapply IHn; eauto. omega. 
-      eu. repeat eexists. eapply vtp_sel. eauto. eauto. eauto. 
+      eu. repeat eexists. eapply vtp_sel. eauto. eauto. eauto. eauto. 
     + SCase "sel2". 
-      eapply stp2_closed2 in H0. simpl in H0. inversion H0. inversion H11. omega.
+      eapply stp2_closed2 in H0. simpl in H0. inversion H0. inversion H12. omega.
     + SCase "and".
       assert (vtpdd m1 G1 x T4). eapply IHn; eauto. omega. eu. 
       assert (vtpdd m1 G1 x T5). eapply IHn; eauto. omega. eu.
@@ -1675,13 +1707,13 @@ Proof.
         eapply stp2_narrow. simpl. eassumption. simpl. eassumption.
       }
       destruct A as [na A].
-      repeat eexists. eapply vtp_fun. eauto. eauto. eauto. eauto. eauto.
+      repeat eexists. eapply vtp_fun. eauto. eauto. eauto. eauto. eauto. eauto. eauto.
       eapply stp2_transf. eauto. eauto. eauto. eauto. eauto. eauto. eauto. reflexivity.
     + SCase "sel2". 
       assert (vtpdd m1 G1 x TX). eapply IHn; eauto. omega. 
-      eu. repeat eexists. eapply vtp_sel. eauto. eauto. eauto. 
+      eu. repeat eexists. eapply vtp_sel. eauto. eauto. eauto. eauto. 
     + SCase "sel2". 
-      eapply stp2_closed2 in H0. simpl in H0. inversion H0. subst. inversion H16. omega.
+      eapply stp2_closed2 in H0. simpl in H0. inversion H0. subst. inversion H17. omega.
     + SCase "and".
       assert (vtpdd m1 G1 x T6). eapply IHn; eauto. omega. eu. 
       assert (vtpdd m1 G1 x T7). eapply IHn; eauto. omega. eu.
@@ -1695,7 +1727,7 @@ Proof.
     + SCase "top". repeat eexists. eapply vtp_top. eapply vtp_closed1. eauto. eauto. 
     + SCase "sel2". 
       assert (vtpdd (S m) G1 x TX). eapply IHn; eauto. omega. 
-      eu. repeat eexists. eapply vtp_sel. eauto. eauto. eauto. 
+      eu. repeat eexists. eapply vtp_sel. eauto. eauto. eauto. eauto.
     + SCase "sel2". 
       eapply stp2_closed2 in H0. simpl in H0. inversion H0. inversion H10. omega.  
     + SCase "bind1".
@@ -1746,14 +1778,14 @@ Proof.
       repeat eexists. eauto. omega. 
   - Case "ssel2". subst. inversion H0; subst; invty.
     + SCase "top". repeat eexists. eapply vtp_top. eapply vtp_closed1. eauto. eauto. 
-    + SCase "ssel1". index_subst. eapply IHn. eauto. eauto. eauto. omega. eauto.
+    + SCase "ssel1". index_subst. index_subst. eapply IHn. eapply H6. eauto. eauto. omega. eauto.
     + SCase "ssel2". 
       assert (vtpdd m1 G1 x TX0). eapply IHn; eauto. omega. 
-      eu. repeat eexists. eapply vtp_sel. eauto. eauto. eauto.
+      eu. repeat eexists. eapply vtp_sel. eauto. eauto. eauto. eauto.
     + SCase "sel1".
-      assert (closed (length ([]:tenv)) (length G1) 0 (TSel (TVar false x0))).
+      assert (closed (length ([]:tenv)) (length G1) 0 (TSel (TVar false x0) l1)) as A.
       eapply stpd2_closed2. eauto.
-      simpl in H7. inversion H7. inversion H12. omega.
+      simpl in A. inversion A. inversion H12. omega.
     + SCase "selx".
       eauto. 
     + SCase "and".
@@ -1768,7 +1800,7 @@ Proof.
     + SCase "top". repeat eexists. eapply vtp_top. eapply vtp_closed1. eauto. eauto. 
     + SCase "sel2". 
       assert (vtpdd m1 G1 x TX). eapply IHn; eauto. omega. 
-      eu. repeat eexists. eapply vtp_sel. eauto. eauto. eauto. 
+      eu. repeat eexists. eapply vtp_sel. eauto. eauto. eauto. eauto. 
     + SCase "sel2". 
       eapply stp2_closed2 in H0. simpl in H0. inversion H0. inversion H13. omega.
     + SCase "and11". eapply IHn in H4. eu. repeat eexists. eauto. omega. eauto. omega. omega. eauto.
@@ -1791,16 +1823,17 @@ Qed.
 (* Reduction semantics  *)
 Inductive step : venv -> tm -> venv -> tm -> Prop :=
 | ST_Obj : forall G1 D,
-    step G1 (tobj D) (vobj (subst_dm (length G1) D)::G1) (tvar true (length G1))
-| ST_AppAbs : forall G1 f x T1 T2 t12,
-    index f G1 = Some (vobj (dfun T1 T2 t12)) ->
-    step G1 (tapp (tvar true f) (tvar true x)) G1 (subst_tm x t12)
-| ST_App1 : forall G1 G1' t1 t1' t2,
+    step G1 (tobj D) (vobj (subst_dms (length G1) D)::G1) (tvar true (length G1))
+| ST_AppAbs : forall G1 f l x ds T1 T2 t12,
+    index f G1 = Some (vobj ds) ->
+    index l (dms_to_list ds) = Some (dfun T1 T2 t12) ->            
+    step G1 (tapp (tvar true f) l (tvar true x)) G1 (subst_tm x t12)
+| ST_App1 : forall G1 G1' t1 t1' l t2,
     step G1 t1 G1' t1' ->
-    step G1 (tapp t1 t2) G1' (tapp t1' t2)
-| ST_App2 : forall G1 G1' f t2 t2',
+    step G1 (tapp t1 l t2) G1' (tapp t1' l t2)
+| ST_App2 : forall G1 G1' f t2 l t2',
     step G1 t2 G1' t2' ->
-    step G1 (tapp (tvar true f) t2) G1' (tapp (tvar true f) t2')
+    step G1 (tapp (tvar true f) l t2) G1' (tapp (tvar true f) l t2')
 .
 
 
@@ -1833,7 +1866,8 @@ Lemma hastp_inv: forall G1 x T n1,
 Proof.
   intros. remember [] as GH. remember (tvar true x) as t.
   induction H; subst; try inversion Heqt.
-  - Case "varx". subst. inversion H0; subst.
+  - Case "varx". subst. admit. (*inversion H0; subst.
+    + repeat eexists. eapply vtp_top. eapply index_max. eauto.
     + assert (stpd2 [] G1 (substt x T11) (substt x T11)) as A. {
         eapply stpd2_refl. eapply closed_subst. eauto.
         econstructor. eapply index_max in H. omega.
@@ -1853,7 +1887,7 @@ Proof.
       eauto. eauto. eauto. eauto. eauto. eauto. eauto. eauto.
       eapply closed_subst. eauto. econstructor. eapply index_max in H. omega.
       eapply closed_subst. eauto. econstructor. eapply index_max in H. omega.
-      eauto.
+      eauto.*)
   - Case "pack". subst.
     destruct IHhas_type. eauto. eauto. ev.
     repeat eexists. eapply vtp_bind. eauto. eauto.
@@ -1864,8 +1898,13 @@ Proof.
     destruct IHhas_type. eauto. eauto. ev.
     assert (exists m0, vtpdd m0 G1 x T2). eexists. eapply vtp_widen; eauto. 
     ev. eu. repeat eexists. eauto. 
-Grab Existential Variables.
-apply 0. apply 0.
+Qed.
+
+Lemma length_subst_dms: forall ds x,
+  (length (dms_to_list ds))=(length (dms_to_list (subst_dms x ds))).
+Proof.
+  intros. induction ds; eauto.
+  simpl. rewrite IHds. reflexivity.
 Qed.
 
 Lemma hastp_subst_aux_z: forall ni, (forall G1 GH TX T x t n1 n2,
@@ -1875,7 +1914,7 @@ Lemma hastp_subst_aux_z: forall ni, (forall G1 GH TX T x t n1 n2,
   (forall G1 GH TX T x ds n1 n2,
   dms_has_type (GH++[TX]) G1 ds T n2 -> n2 < ni ->
   has_type [] G1 (tvar true x) (substt x TX) n1 ->
-  exists n3, dms_has_type (map (substt x) GH) G1 (subst_dm x ds) (substt x T) n3).
+  exists n3, dms_has_type (map (substt x) GH) G1 (subst_dms x ds) (substt x T) n3).
 Proof.
   intro ni. induction ni. split; intros; omega. destruct IHni as [IHniT IHniD].
   split;
@@ -2002,16 +2041,22 @@ Proof.
     edestruct stp2_subst_narrow_z. eapply H3. eapply HV.
     edestruct IHniT as [? IH]. eapply H2. omega. eauto.
     eexists. eapply T_Sub. eauto. eauto.
+  - Case "dnil". subst. simpl.
+    eexists. eapply D_Nil.
   - Case "mem". subst. simpl.
-    eexists. eapply D_Mem. eapply closed_subst0. rewrite app_length in H2. rewrite map_length. eauto. eapply has_type_closed1. eauto.
+    edestruct IHniD as [? IH]. eapply H2. omega. eauto.
+    eexists. eapply D_Mem. eauto. eapply closed_subst0. rewrite app_length in H3. rewrite map_length. eauto. eapply has_type_closed1. eauto. eauto.
+    unfold substt. simpl. rewrite <- length_subst_dms. reflexivity.
   - Case "abs". subst. simpl.
+    edestruct IHniD as [? IHD]. eapply H2. omega. eauto.
     edestruct IHniT with (GH:=T11::GH1) as [? HI] . eauto. omega. eauto.
     simpl in HI. 
-    eexists. eapply D_Abs. eapply HI.
+    eexists. eapply D_Abs. eapply IHD. eapply HI.
     rewrite map_length. rewrite app_length. simpl.
     rewrite subst_open. unfold substt. reflexivity.
-    eapply closed_subst0. rewrite map_length. rewrite app_length in H4. simpl in H4. eauto. eauto. eapply has_type_closed1. eauto.
-    eapply closed_subst0. rewrite map_length. rewrite app_length in H5. simpl in H5. eauto. eapply has_type_closed1. eauto.
+    eapply closed_subst0. rewrite map_length. rewrite app_length in H5. simpl in H5. eauto. eauto. eapply has_type_closed1. eauto.
+    eapply closed_subst0. rewrite map_length. rewrite app_length in H6. simpl in H6. eauto. eapply has_type_closed1. eauto. eauto.
+    unfold substt. simpl. rewrite <- length_subst_dms. reflexivity.
 Grab Existential Variables.
 apply 0. apply 0.
 Qed.
@@ -2069,48 +2114,48 @@ Proof.
     simpl. rewrite subst_open_commute0b. erewrite subst_closed_id. reflexivity. eauto.
     eapply closed_extend. eauto.
   - Case "app". subst.
-    assert (closed (length ([]:tenv)) (length G1) 0 (TFun T1 T)) as TF. eapply has_type_closed. eauto. 
+    assert (closed (length ([]:tenv)) (length G1) 0 (TFun l T1 T)) as TF. eapply has_type_closed. eauto. 
     assert ((exists x : id, t2 = tvar true x) \/
                 (exists (G' : venv) (t' : tm) n2,
                    step G1 t2 (G'++G1) t' /\ has_type [] (G'++G1) t' T1 n2)) as HX.
     eapply IHhas_type2. eauto. eauto. eauto. inversion TF. eauto. 
     assert ((exists x : id, t1 = tvar true x) \/
                 (exists (G' : venv) (t' : tm) n2,
-                   step G1 t1 (G'++G1) t' /\ has_type [] (G'++G1) t' (TFun T1 T) n2)) as HF.
+                   step G1 t1 (G'++G1) t' /\ has_type [] (G'++G1) t' (TFun l T1 T) n2)) as HF.
     eapply IHhas_type1. eauto. eauto. eauto. eauto.
     destruct HF.
     + SCase "fun-val".
       destruct HX.
       * SSCase "arg-val".
         ev. ev. subst. 
-        assert (exists m n1, vtp m G1 x (TFun T1 T) n1). eapply hastp_inv. eauto.
+        assert (exists m n1, vtp m G1 x (TFun l T1 T) n1). eapply hastp_inv. eauto.
         assert (exists m n1, vtp m G1 x0 T1 n1). eapply hastp_inv. eauto.
         ev. inversion H2. subst.
         assert (vtpdd x1 G1 x0 T0). eapply vtp_widen. eauto. eauto. eauto. eauto. eauto.
         eu.
-        assert (exists T, (exists n1, has_type [] G1 (tvar true x) T n1) /\ substt x T' = T) as A. eexists. split. eexists. eapply T_Varx. eauto. eauto. eauto. eauto. eapply closed_subst. eapply dms_has_type_closed in H7. eauto. econstructor. eapply index_max in H6. omega. reflexivity.
+        assert (exists T, (exists n1, has_type [] G1 (tvar true x) T n1) /\ substt x T' = T) as A. eexists. split. eexists. eapply T_Varx. eauto. eauto. eauto. eauto. eapply closed_subst. eapply dms_has_type_closed in H10. eauto. econstructor. eapply index_max in H7. omega. reflexivity.
         destruct A as [Tx [[na A] EqTx]].
         assert (has_typed (map (substt x) [T1x]) G1 (subst_tm x tx) (substt x (open 0 (TVar false 1) T2x))) as HIx.
-        eapply hastp_subst_z. eapply H10. rewrite EqTx. eapply A.
+        eapply hastp_subst_z. eapply H13. rewrite EqTx. eapply A.
         eu. simpl in HIx.
         assert (has_typed (map (substt x0) []) G1 (subst_tm x0 (subst_tm x tx)) (substt x0 (substt x (open 0 (TVar false 1) T2x)))) as HIx0.
-        eapply hastp_subst. rewrite app_nil_l. eapply HIx. simpl in H8. inversion H8. unfold substt. rewrite H12. eauto.
+        eapply hastp_subst. rewrite app_nil_l. eapply HIx. simpl in H11. inversion H11. unfold substt. rewrite H9. eauto.
         eu. simpl in HIx0.
         assert ((substt x (open 0 (TVar false 1) T2x))=(open 0 (TVar false 0) (substt x T2x))) as EqT2x. {
           change 1 with (0+1). rewrite subst_open. reflexivity.
         }
         assert (has_typed [] G1 (subst_tm x0 t) (substt x0 (open 0 (TVar false 0) T2))) as HI. {
-          inversion H8; subst. unfold substt in EqT2x. rewrite <- EqT2x. eauto.
+          inversion H11; subst. unfold substt in EqT2x. rewrite <- EqT2x. eauto.
         }
         eu. simpl in HI.
-        edestruct stp2_subst_narrow as [? HI2]. rewrite app_nil_l. eapply H20. eauto.
+        edestruct stp2_subst_narrow as [? HI2]. rewrite app_nil_l. eapply H23. eauto.
         simpl in HI2.
         assert (substt x0 (open 0 (TVar false 0) T) = T) as EqT. {
           erewrite <- closed_no_open. erewrite subst_closed_id. reflexivity.
           eassumption. eassumption.
         }
         rewrite EqT in HI2.
-        right. repeat eexists. rewrite app_nil_l. eapply ST_AppAbs. eauto.
+        right. repeat eexists. rewrite app_nil_l. eapply ST_AppAbs. eauto. eauto.
         eapply T_Sub. eauto. eauto.
       * SSCase "arg_step".
         ev. subst. 
@@ -2123,7 +2168,7 @@ Proof.
       simpl in *. rewrite app_length. eapply closed_extend_mult. eassumption. omega.
 
   - Case "appvar". subst.
-    assert (closed (length ([]:tenv)) (length G1) 0 (TFun T1 T2)) as TF. eapply has_type_closed. eauto.
+    assert (closed (length ([]:tenv)) (length G1) 0 (TFun l T1 T2)) as TF. eapply has_type_closed. eauto.
     assert ((exists x : id, tvar b2 x2 = tvar true x) \/
                 (exists (G' : venv) (t' : tm) n2,
                    step G1 (tvar b2 x2) (G'++G1) t' /\ has_type [] (G'++G1) t' T1 n2)) as HX.
@@ -2136,39 +2181,39 @@ Proof.
     clear HX. subst b2.
     assert ((exists x : id, t1 = tvar true x) \/
                 (exists (G' : venv) (t' : tm) n2,
-                   step G1 t1 (G'++G1) t' /\ has_type [] (G'++G1) t' (TFun T1 T2) n2)) as HF.
+                   step G1 t1 (G'++G1) t' /\ has_type [] (G'++G1) t' (TFun l T1 T2) n2)) as HF.
     eapply IHhas_type1. eauto. eauto. eauto. eauto.
     destruct HF.
     + SCase "fun-val".
       ev. ev. subst.
-      assert (exists m n1, vtp m G1 x (TFun T1 T2) n1). eapply hastp_inv. eauto.
+      assert (exists m n1, vtp m G1 x (TFun l T1 T2) n1). eapply hastp_inv. eauto.
       assert (exists m n1, vtp m G1 x2 T1 n1). eapply hastp_inv. eauto.
       ev. inversion H1. subst.
       assert (vtpdd x0 G1 x2 T0). eapply vtp_widen. eauto. eauto. eauto. eauto. eauto.
       eu.
-      assert (exists T, (exists n1, has_type [] G1 (tvar true x) T n1) /\ substt x T' = T) as A. eexists. split. eexists. eapply T_Varx. eauto. eauto. eauto. eauto. eapply closed_subst. eapply dms_has_type_closed in H7. eauto. econstructor. eapply index_max in H6. omega. reflexivity.
+      assert (exists T, (exists n1, has_type [] G1 (tvar true x) T n1) /\ substt x T' = T) as A. eexists. split. eexists. eapply T_Varx. eauto. eauto. eauto. eauto. eapply closed_subst. eapply dms_has_type_closed in H10. eauto. econstructor. eapply index_max in H7. omega. reflexivity.
       destruct A as [Tx [[na A] EqTx]].
       assert (has_typed (map (substt x) [T1x]) G1 (subst_tm x tx) (substt x (open 0 (TVar false 1) T2x))) as HIx.
-      eapply hastp_subst_z. eapply H10. rewrite EqTx. eapply A.
+      eapply hastp_subst_z. eapply H13. rewrite EqTx. eapply A.
       eu. simpl in HIx.
       assert (has_typed (map (substt x2) []) G1 (subst_tm x2 (subst_tm x tx)) (substt x2 (substt x (open 0 (TVar false 1) T2x)))) as HIx0.
-      eapply hastp_subst. rewrite app_nil_l. eapply HIx. simpl in H8. inversion H8. unfold substt. rewrite H12. eauto.
+      eapply hastp_subst. rewrite app_nil_l. eapply HIx. simpl in H11. inversion H11. unfold substt. rewrite H9. eauto.
       eu. simpl in HIx0.
       assert ((substt x (open 0 (TVar false 1) T2x))=(open 0 (TVar false 0) (substt x T2x))) as EqT2x. {
         change 1 with (0+1). rewrite subst_open. reflexivity.
       }
       assert (has_typed [] G1 (subst_tm x2 t) (substt x2 (open 0 (TVar false 0) T3))) as HI. {
-        inversion H8; subst. unfold substt in EqT2x. rewrite <- EqT2x. eauto.
+        inversion H11; subst. unfold substt in EqT2x. rewrite <- EqT2x. eauto.
       }
       eu. simpl in HI.
-      edestruct stp2_subst_narrow as [? HI2]. rewrite app_nil_l. eapply H20. eauto.
+      edestruct stp2_subst_narrow as [? HI2]. rewrite app_nil_l. eapply H23. eauto.
       simpl in HI2.
       assert ((substt x2 (open 0 (TVar false 0) T2))=(open 0 (TVar true x2) T2)) as EqT2. {
         rewrite subst_open_commute0b. erewrite subst_closed_id. reflexivity.
         eassumption.
       }
       rewrite EqT2 in HI2.
-      right. repeat eexists. rewrite app_nil_l. eapply ST_AppAbs. eauto.
+      right. repeat eexists. rewrite app_nil_l. eapply ST_AppAbs. eauto. eauto.
       eapply T_Sub. eauto. eauto.
     + SCase "fun_step".
       ev. subst. right. repeat eexists. eapply ST_App1. eauto. eapply T_AppVar.
